
% Author: Kimberly Golubeva
% Date: 28 September 2020
%Revised LD April 2021
% Lauren DeDieu, Jerrod M.~Smith, Kimberly Golubeva and Christian Bagshaw
% A Resource Bank for Writing Intensive Mathematics Courses
% This work is licensed under a  Creative Commons Attribution-NonCommercial-ShareAlike 4.0 International License
% http://creativecommons.org/licenses/by-nc-sa/4.0/
\section{Factoring Complex Polynomials}

\begin{xca}{xca:factor_complex_poly}
For each of the following polynomials $p(z)$.  Prove that there exists a polynomial $h(z)$ such that \[p(z) = (z-z_0)h(z) + p(z_0).\]
\begin{itemize}
    \item $p(z) = z^2$  and $z_0 = i$\;,
    \item $p(z) = z^3 + z^2 + z$ and $z_0=-1$\;.
\end{itemize}
\end{xca}

\begin{flaw}{flaw:factor_complex_poly} %change the label
First, we find $h(z)$ when $p(z) = z^2$  and $z_0 = i$\;:
\begin{align*}
    p(z) &= (z - z_0)h(z) + p(z_0) \\
    &= (z + i)h(z) + p(i) \\
    &= (z + i)h(z) - 1 \\
    &= (z + i)(z - i) - 1 \\
    &= z^2 - zi + zi - i^2 - 1 \\
    &= z^2 + 1 -1 \\
    &= z^2\;,
\end{align*}
and so $h(z) = z-i\;.$

\noindent Next, we find $h(z)$ when $p(z) = z^3 + z^2 + z$  and $z_0 = -1$\;:
\begin{align*}
    p(z) &= (z - z_0)h(z) + p(z_0) \\
    &= (z + 1)h(z) + p(-1) \\
    &= (z + 1)(z^2 +1) - 1 \\
    &= z^3 + z^2 +z +1 -1\\
    &= z^3 + z^2 +z\;,
\end{align*}
and so $h(z) = z^2+1\;.$
\end{flaw}

\clearpage
\subsection{Error classification}

%Provide a brief classification and explanation of the errors in the Flawed Proof \ref{flaw:proof1}. %change the label

There are several errors
% is only one error ... etc.
 in the Flawed Proof \ref{flaw:factor_complex_poly}. %change the label


 \begin{description}
 	\item[N-FS:] There is an apparent typo in the first calculation: the polynomial $p(z)$ should be written as $p(z) = (z - i)h(z) + p(i)$ as opposed to $p(z) = (z + i)h(z) + p(i).$
 	\item[N-Log:] In the first calculation, they use $h(z) = z-i$ and then claim that their calculation implies that $h(z) = z-i$. A similar mistake is made in the second calculation.
 \end{description}


\subsubsection{Error codes}
\begin{itemize}
	\item 	Novice False Statement (N-FS)
	\item   Novice Logical Order (N-Log)
\end{itemize}
See Section \ref{sec-error} for more information about error classifications.

\clearpage
\subsection{Corrected proof}

The following is a corrected version of Flawed Proof \ref{flaw:factor_complex_poly}. %change the label

\begin{prf}{prf:factor_complex_poly} %change the label
First consider $p(z) = z^2$  and $z_0 = i$.  Choose $h(z) = z+i$. Indeed, if $h(z) = z+i$, then we have

\begin{align*}
    p(z) &= (z - z_0)h(z) + p(z_0) \\
    &= (z - i)(z+i) + p(i) \\
    &= (z - i)(z +i) - 1 \\
    &= z^2 - zi + zi - i^2 - 1 \\
    &= z^2 + 1 -1 \\
    &= z^2\;.
\end{align*}

Now, consider $p(z) = z^3 + z^2 + z$  and $z_0 = -1$.  Choose $h(z) = z^2+1$. Indeed, if $h(z) = z^2+1$ then we have:

\begin{align*}
    p(z) &= (z - z_0)h(z) + p(z_0) \\
    &= (z + 1)(z^2+1) + p(-1) \\
    &= (z + 1)(z^2 +1) - 1 \\
    &= z^3 + z^2 +z +1 -1\\
    &= z^3 + z^2 +z\;.
\end{align*}
\end{prf}
