% Author: Kimberly Golubeva
% Date: 25 August 2020
%Revised LD April 2021
% Lauren DeDieu, Jerrod M.~Smith, Kimberly Golubeva and Christian Bagshaw
% A Resource Bank for Writing Intensive Mathematics Courses
% This work is licensed under a  Creative Commons Attribution-NonCommercial-ShareAlike 4.0 International License
% http://creativecommons.org/licenses/by-nc-sa/4.0/
\section{Definition of an Infinite Limit}

\begin{xca}{xca:root_limit}
Let $n \in \Z$. Prove that
$$\lim_{n \rightarrow \infty} \sqrt{4n^2-1} - 2n = 0.$$
\end{xca}

\begin{flaw}{flaw:root_limit} %change the label
\begin{align*}
    \lim_{n \rightarrow \infty} \sqrt{4n^2-1} - 2n &= \lim_{n \rightarrow \infty} \sqrt{4n^2} - 2n \\
    &= \lim_{n \rightarrow \infty} 2n - 2n \\
    &= 0
\end{align*}
\end{flaw}

\clearpage
\subsection{Error classification}

%Provide a brief classification and explanation of the errors in the Flawed Proof \ref{flaw:proof1}. %change the label

There are several errors
% is only one error ... etc.
 in the Flawed Proof \ref{flaw:root_limit}. %change the label


 \begin{description}
 	\item[EO-(WM):] Omitted crucial steps of the proof due to a misunderstanding that to ``prove'' in this context means to use the formal $\varepsilon$ definition of an infinite limit.
 	\item[C-A:] The equality $\displaystyle\lim_{n \rightarrow \infty} \sqrt{4n^2-1} - 2n = \lim_{n \rightarrow \infty} \sqrt{4n^2} - 2n$ requires justification.
 \end{description}

\subsubsection{Error codes}
\begin{itemize}
	\item 	Error-Caused Omission due Wrong Method (EO-(WM))
	\item   Content Assertion (C-A)
\end{itemize}
See Section \ref{sec-error} for more information about error classifications.

\clearpage
\subsection{Corrected proof}

The following is a corrected version of Flawed Proof \ref{flaw:root_limit}. %change the label

\begin{prf}{prf:root_limit} %change the label
Suppose $n \in \Z$. Fix $\varepsilon > 0.$ Choose $N \in \mathbb{N}$ such that $N> \frac{1}{2\varepsilon}$. Then for $n \geq N,$ we have:

 \begin{align*}
    \left | \sqrt{4n^2-1} - 2n - 0 \right | &= \left | \left(\sqrt{4n^2-1} - 2n\right) \frac{\sqrt{4n^2-1} + 2n}{\sqrt{4n^2-1} + 2n}\right | \\
    &= \left | \frac{(4n^2-1)-4n^2}{\sqrt{4n^2-1}+2n} \right | \\
    &= \left |\frac{-1}{\sqrt{4n^2-1} + 2n} \right | \\
    &=\frac{1}{\sqrt{4n^2-1} + 2n} \\
    &\leq \frac{1}{2n}\;,
 \end{align*}

since $\sqrt{4n^2-1}\geq 0 \Rightarrow \sqrt{4n^2-1}+2n\geq 2n \Rightarrow \dfrac{1}{2n}\geq \dfrac{1}{\sqrt{4n^2-1}+2n}$. \\

Hence, we have

$$ \left| \sqrt{4n^2-1} - 2n - 0 \right | \leq \frac{1}{2n} \leq \frac{1}{2N} < \varepsilon\;.$$ \\

Note that the second inequality follows from the fact that $n\geq N$ implies that $\frac{1}{2N}\geq\frac{1}{2n}$. The third inequality follows from the fact that $N> \frac{1}{2\varepsilon}$ implies that $\frac1{2N} < \varepsilon$. \\

Thus, $\displaystyle \lim_{n \rightarrow \infty} \sqrt{4n^2-1} - 2n = 0$ by the definition of convergence.
\end{prf} 