% Author: Kimberly Golubeva
% Date: 27 July 2020
% Revised: JMS 3 Feb 2021
% Lauren DeDieu, Jerrod M.~Smith, Kimberly Golubeva and Christian Bagshaw
% A Resource Bank for Writing Intensive Mathematics Courses
% This work is licensed under a  Creative Commons Attribution-NonCommercial-ShareAlike 4.0 International License
% http://creativecommons.org/licenses/by-nc-sa/4.0/
\section{Summation Formula Induction}

\begin{xca}{xca:sum_induction}
Prove that
$$\sum_{i=1}^n i = \frac{n(n+1)}{2}\;,$$
 for all integers $n \geq 1.$
\end{xca}


\begin{flaw}{flaw:sum_induction} 
\textbf{Base Case (n=1):} 
\begin{align*}
    \sum_{i=1}^1 i & = \frac{1+(1+1)}{2} \\
    1 &= \frac{2}{2} \\
    1 &= 1
\end{align*}
\textbf{Induction Hypothesis:} Suppose that $k \geq 1$ is an integer and that 
$$\sum_{i=1}^k i = \frac{k(k+1)}{2}\;.$$ Then
$$\sum_{i=1}^{k+1} i = \frac{(k+1)(k+2)}{2}\;.$$
So
\begin{align*}
    \sum_{i=1}^{k+1} i &= \left(\sum_{i=1}^k i\right) + (k+1) \\
    &= \frac{k(k+1)}{2} + (k+1) & (\text{by the IH})\\
    &= \frac{k(k+1) + 2(k+1)}{2} \\
    &= \frac{(k+1)(k+2)}{2}\;.
\end{align*}
Thus, 
$$\sum_{i=1}^n i = \frac{n(n+1)}{2}\;,$$
 for all integers $n \geq 1.$
\end{flaw}

\clearpage
\subsection{Error classification}


There are several errors
% is only one error ... etc.
 in the Flawed Proof \ref{flaw:sum_induction}. 

 
 \begin{description}
 	\item[C-FI/C-A:] The base contains a false implication.  Moreover, the base case begins with the assertion of what needs to be shown.
 	\item[C-A:] The induction hypothesis contains the assertion of the induction step.
 \end{description}

 
\subsubsection{Error codes}
\begin{itemize}
	\item 	Content False Implication (C-FI)
	\item   Content Assertion (C-A)
\end{itemize}
See Section \ref{sec-error} for more information about error classifications.

\clearpage
\subsection{Corrected proof}

The following is a corrected version of Flawed Proof \ref{flaw:sum_induction}. 

\begin{prf}{prf:sum_induction} 
Suppose that $n$ is an integer and $n\geq 1$.

\noindent \textbf{Base Case (n=1):} Suppose $n=1$. Then
$$\sum_{i=1}^1 i = 1 = \frac{2}{2} = \frac{1(2)}{2} = \frac{1(1+1)}{2}.$$ 
\textbf{Induction Hypothesis:} Suppose that $k \geq 1$ is an integer and that 
$$\sum_{i=1}^k i = \frac{k(k+1)}{2}\;.$$
We want to prove that 
$$\sum_{i=1}^{k+1} i = \frac{(k+1)(k+2)}{2}\;.$$
It follows that 
\begin{align*}
    \sum_{i=1}^{k+1} i &= \left(\sum_{i=1}^k i\right) + (k+1) \\
    &= \frac{k(k+1)}{2} + (k+1)  & (\text{by the induction hypothesis})\\
    &= \frac{k(k+1) + 2(k+1)}{2} \\
    &= \frac{(k+1)(k+2)}{2}\;.
\end{align*}
Thus, by induction, 
$$\sum_{i=1}^n i = \frac{n(n+1)}{2}\;,$$
 for all integers $n \geq 1.$
\end{prf}
